deps/poulet4/lib/P4automata/Benchmarks/Edge.v
@@ -13,196 +13,222 @@ Require Import Coq.Program.Equality.
 
 Open Scope p4a.
 
-Notation eth_size := 112.
-Notation mpls_size := 32.
-Notation eompls_size := 32.
-Notation ipv4_size := 156.
-Notation ipv6_size := 316.
+Module Plain.
+  Notation eth_size := 112.
+  Notation mpls_size := 32.
+  Notation eompls_size := 32.
+  Notation ipv4_size := 156.
+  Notation ipv6_size := 316.
 
-Inductive header: nat -> Type :=
-| HdrEth0: header eth_size
-| HdrEth1: header eth_size
-| HdrMPLS0: header mpls_size
-| HdrMPLS1: header mpls_size
-| HdrEoMPLS: header eompls_size
-| HdrIPVer: header 4
-| HdrIPv4: header ipv4_size
-| HdrIPv6: header ipv6_size.
+  Inductive header: nat -> Type :=
+  | HdrEth0: header eth_size
+  | HdrEth1: header eth_size
+  | HdrMPLS0: header mpls_size
+  | HdrMPLS1: header mpls_size
+  | HdrEoMPLS: header eompls_size
+  | HdrIPVer: header 4
+  | HdrIPv4: header ipv4_size
+  | HdrIPv6: header ipv6_size.
 
-Derive Signature for header.
-Definition h32_eq_dec (x y: header 32) : {x = y} + {x <> y}.
-refine (
-  match x with
-  | HdrMPLS0 =>
-    match y with
-    | HdrMPLS0 => left eq_refl
-    | HdrMPLS1 => right _
-    | HdrEoMPLS => right _
+  Derive Signature for header.
+  Definition h32_eq_dec (x y: header 32) : {x = y} + {x <> y}.
+  refine (
+    match x with
+    | HdrMPLS0 =>
+      match y with
+      | HdrMPLS0 => left eq_refl
+      | HdrMPLS1 => right _
+      | HdrEoMPLS => right _
+      end
+    | HdrMPLS1 =>
+      match y with
+      | HdrMPLS0 => right _
+      | HdrMPLS1 => left eq_refl
+      | HdrEoMPLS => right _
+      end
+    | HdrEoMPLS =>
+      match y with
+      | HdrMPLS0 => right _
+      | HdrMPLS1 => right _
+      | HdrEoMPLS => left eq_refl
+      end
     end
-  | HdrMPLS1 =>
-    match y with
-    | HdrMPLS0 => right _
-    | HdrMPLS1 => left eq_refl
-    | HdrEoMPLS => right _
+  ); unfold "<>"; intros H; inversion H.
+  Defined.
+  Definition h4_eq_dec (x y: header 4) : {x = y} + {x <> y}.
+  refine (
+    match x with
+    | HdrIPVer =>
+      match y with
+      | HdrIPVer => left eq_refl
+      end
     end
-  | HdrEoMPLS =>
-    match y with
-    | HdrMPLS0 => right _
-    | HdrMPLS1 => right _
-    | HdrEoMPLS => left eq_refl
+  ); unfold "<>"; intros H; inversion H.
+  Defined.
+  Definition h112_eq_dec (x y: header 112) : {x = y} + {x <> y}.
+  refine (
+    match x with
+    | HdrEth0 =>
+      match y with
+      | HdrEth0 => left eq_refl
+      | HdrEth1 => right _
+      end
+    | HdrEth1 =>
+      match y with
+      | HdrEth0 => right _
+      | HdrEth1 => left eq_refl
+      end
     end
-  end
-); unfold "<>"; intros H; inversion H.
-Defined.
-Definition h4_eq_dec (x y: header 4) : {x = y} + {x <> y}.
-refine (
-  match x with
-  | HdrIPVer =>
-    match y with
-    | HdrIPVer => left eq_refl
+  ); unfold "<>"; intros H; inversion H.
+  Defined.
+  Definition h316_eq_dec (x y: header 316) : {x = y} + {x <> y}.
+  refine (
+    match x with
+    | HdrIPv6 =>
+      match y with
+      | HdrIPv6 => left eq_refl
+      end
     end
-  end
-); unfold "<>"; intros H; inversion H.
-Defined.
-Definition h112_eq_dec (x y: header 112) : {x = y} + {x <> y}.
-refine (
-  match x with
-  | HdrEth0 =>
-    match y with
-    | HdrEth0 => left eq_refl
-    | HdrEth1 => right _
+  ); unfold "<>"; intros H; inversion H.
+  Defined.
+  Definition h156_eq_dec (x y: header 156) : {x = y} + {x <> y}.
+  refine (
+    match x with
+    | HdrIPv4 =>
+      match y with
+      | HdrIPv4 => left eq_refl
+      end
     end
-  | HdrEth1 =>
-    match y with
-    | HdrEth0 => right _
-    | HdrEth1 => left eq_refl
-    end
-  end
-); unfold "<>"; intros H; inversion H.
-Defined.
-Definition h316_eq_dec (x y: header 316) : {x = y} + {x <> y}.
-refine (
-  match x with
-  | HdrIPv6 =>
-    match y with
-    | HdrIPv6 => left eq_refl
-    end
-  end
-); unfold "<>"; intros H; inversion H.
-Defined.
-Definition h156_eq_dec (x y: header 156) : {x = y} + {x <> y}.
-refine (
-  match x with
-  | HdrIPv4 =>
-    match y with
-    | HdrIPv4 => left eq_refl
-    end
-  end
-); unfold "<>"; intros H; inversion H.
-Defined.
-Definition header_eqdec_ (n: nat) (x: header n) (y: header n) : {x = y} + {x <> y}.
-  solve_header_eqdec_ n x y
-    ((existT (fun n => forall x y: header n, {x = y} + {x <> y}) _ h32_eq_dec) ::
-     (existT _ _ h4_eq_dec) ::
-     (existT _ _ h112_eq_dec) ::
-     (existT _ _ h316_eq_dec) ::
-     (existT _ _ h156_eq_dec) ::
-      nil).
-Defined.
+  ); unfold "<>"; intros H; inversion H.
+  Defined.
+  Definition header_eqdec_ (n: nat) (x: header n) (y: header n) : {x = y} + {x <> y}.
+    solve_header_eqdec_ n x y
+      ((existT (fun n => forall x y: header n, {x = y} + {x <> y}) _ h32_eq_dec) ::
+      (existT _ _ h4_eq_dec) ::
+      (existT _ _ h112_eq_dec) ::
+      (existT _ _ h316_eq_dec) ::
+      (existT _ _ h156_eq_dec) ::
+        nil).
+  Defined.
 
-Global Instance header_eqdec: forall n, EquivDec.EqDec (header n) eq := header_eqdec_.
-Global Instance header_eqdec': EquivDec.EqDec (Syntax.H' header) eq.
-  solve_eqdec'.
-Defined.
-Global Instance header_finite: forall n, @Finite (header n) _ _.
-  intros n; solve_indexed_finiteness n [32; 4 ; 112 ; 316 ; 156 ].
-Qed.
+  Global Instance header_eqdec: forall n, EquivDec.EqDec (header n) eq := header_eqdec_.
+  Global Instance header_eqdec': EquivDec.EqDec (Syntax.H' header) eq.
+    solve_eqdec'.
+  Defined.
+  Global Instance header_finite: forall n, @Finite (header n) _ _.
+    intros n; solve_indexed_finiteness n [32; 4 ; 112 ; 316 ; 156 ].
+  Qed.
 
-Global Program Instance header_finite': @Finite {n & header n} _ header_eqdec' :=
-  {| enum := [
-      existT _ _ HdrEth0
-    ; existT _ _ HdrEth1
-    ; existT _ _ HdrMPLS0
-    ; existT _ _ HdrMPLS1
-    ; existT _ _ HdrEoMPLS
-    ; existT _ _ HdrIPVer
-    ; existT _ _ HdrIPv4
-    ; existT _ _ HdrIPv6
-    ] |}.
-Next Obligation.
-  solve_header_finite.
-Qed.
-Next Obligation.
-dependent destruction X; subst;
-repeat (
-  match goal with
-  | |- ?L \/ ?R => (now left; trivial) || right
-  end
-).
-Qed.
+  Global Program Instance header_finite': @Finite {n & header n} _ header_eqdec' :=
+    {| enum := [
+        existT _ _ HdrEth0
+      ; existT _ _ HdrEth1
+      ; existT _ _ HdrMPLS0
+      ; existT _ _ HdrMPLS1
+      ; existT _ _ HdrEoMPLS
+      ; existT _ _ HdrIPVer
+      ; existT _ _ HdrIPv4
+      ; existT _ _ HdrIPv6
+      ] |}.
+  Next Obligation.
+    solve_header_finite.
+  Qed.
+  Next Obligation.
+  dependent destruction X; subst;
+  repeat (
+    match goal with
+    | |- ?L \/ ?R => (now left; trivial) || right
+    end
+  ).
+  Qed.
 
-Inductive state: Type :=
-| ParseEth0
-| ParseEth1
-| ParseMPLS0
-| ParseMPLS1
-| ParseEoMPLS
-| ParseIPVer
-| ParseIPv4
-| ParseIPv6.
+  Inductive state: Type :=
+  | ParseEth0
+  | ParseEth1
+  | ParseMPLS0
+  | ParseMPLS1
+  | ParseEoMPLS
+  | ParseIPVer
+  | ParseIPv4
+  | ParseIPv6.
 
-Definition states (s: state) : P4A.state state header :=
-  match s with
-  | ParseEth0 =>
-    {| st_op := extract(HdrEth0);
-       st_trans := transition select (| (EHdr HdrEth0)[111--96] |)
-                              {{ [| hexact 0x8847 |] ==> inl ParseMPLS0 ;;;
-                                 [| hexact 0x8848 |] ==> inl ParseMPLS0 ;;;
-                                 [| hexact 0x0800 |] ==> inl ParseIPv4 ;;;
-                                 [| hexact 0x86dd |] ==> inl ParseIPv6 ;;;
-                                 reject }}
-    |}
-  | ParseMPLS0 => 
-    {| st_op := extract(HdrMPLS0);
-       st_trans := transition select (| (EHdr HdrMPLS0)[24--24] |)
-                              {{ [| hexact 0 |] ==> inl ParseMPLS1 ;;;
-                                 [| hexact 1 |] ==> inl ParseIPVer ;;;
-                                 reject
-                              }}
-    |}
-  | ParseMPLS1 => 
-    {| st_op := extract(HdrMPLS1);
-       st_trans := transition (inl ParseIPVer)
-    |}
-  | ParseIPVer =>
-    {| st_op := extract(HdrIPVer);
-       st_trans := transition select (| EHdr HdrIPVer |)
-                              {{ [| exact #b|0|0|0|0 |] ==> inl ParseEoMPLS;;;
-                                 [| exact #b|0|1|0|0 |] ==> inl ParseIPv4;;;
-                                 [| exact #b|0|1|1|0 |] ==> inl ParseIPv6;;;
-                                 reject
-                              }}
-    |}
-  | ParseEoMPLS =>
-    {| st_op := extract(HdrEoMPLS);
-       st_trans := transition (inl ParseEth1) |}
-  | ParseIPv4 =>
-    {| st_op := extract(HdrIPv4);
-       st_trans := transition accept |}
-  | ParseIPv6 =>
-    {| st_op := extract(HdrIPv6);
-       st_trans := transition accept |}
-  | ParseEth1 =>
-    {| st_op := extract(HdrEth1);
-       st_trans := transition accept |}
-  end.
+  Definition states (s: state) : P4A.state state header :=
+    match s with
+    | ParseEth0 =>
+      {| st_op := extract(HdrEth0);
+        st_trans := transition select (| (EHdr HdrEth0)[111--96] |)
+                                {{[| exact #b|1|0|0|0|1|0|0|0|0|1|0|0|0|1|1|1 |] ==> inl ParseMPLS0 ;;;
+                                  [| exact #b|1|0|0|0|1|0|0|0|0|1|0|0|1|0|0|0 |] ==> inl ParseMPLS0 ;;;
+                                  [| exact #b|0|0|0|0|1|0|0|0|0|0|0|0|0|0|0|0 |] ==> inl ParseIPv4 ;;;
+                                  [| exact #b|1|0|0|0|0|1|1|0|1|1|0|1|1|1|0|1 |] ==> inl ParseIPv6 ;;;
+                                  reject }}
+      |}
+    | ParseMPLS0 => 
+      {| st_op := extract(HdrMPLS0);
+        st_trans := transition select (| (EHdr HdrMPLS0)[24--24] |)
+                                {{ [| hexact 0 |] ==> inl ParseMPLS1 ;;;
+                                  [| hexact 1 |] ==> inl ParseIPVer ;;;
+                                  reject
+                                }}
+      |}
+    | ParseMPLS1 => 
+      {| st_op := extract(HdrMPLS1);
+        st_trans := transition (inl ParseIPVer)
+      |}
+    | ParseIPVer =>
+      {| st_op := extract(HdrIPVer);
+        st_trans := transition select (| EHdr HdrIPVer |)
+                                {{ [| exact #b|0|0|0|0 |] ==> inl ParseEoMPLS;;;
+                                  [| exact #b|0|1|0|0 |] ==> inl ParseIPv4;;;
+                                  [| exact #b|0|1|1|0 |] ==> inl ParseIPv6;;;
+                                  reject
+                                }}
+      |}
+    | ParseEoMPLS =>
+      {| st_op := extract(HdrEoMPLS);
+        st_trans := transition (inl ParseEth1) |}
+    | ParseIPv4 =>
+      {| st_op := extract(HdrIPv4);
+        st_trans := transition accept |}
+    | ParseIPv6 =>
+      {| st_op := extract(HdrIPv6);
+        st_trans := transition accept |}
+    | ParseEth1 =>
+      {| st_op := extract(HdrEth1);
+        st_trans := transition accept |}
+    end.
 
 
 
+  Scheme Equality for state.
+  Global Instance state_eqdec: EquivDec.EqDec state eq := state_eq_dec.
+  Global Program Instance state_finite: @Finite state _ state_eq_dec :=
+    {| enum := [ParseEth0; ParseEth1; ParseMPLS0; ParseMPLS1; ParseEoMPLS; ParseIPVer; ParseIPv4; ParseIPv6] |}.
+  Next Obligation.
+  repeat constructor;
+    repeat match goal with
+            | H: List.In _ [] |- _ => apply List.in_nil in H; exfalso; exact H
+            | |- ~ List.In _ [] => apply List.in_nil
+            | |- ~ List.In _ (_ :: _) => unfold not; intros
+            | H: List.In _ (_::_) |- _ => inversion H; clear H
+            | _ => discriminate
+            end.
+  Qed.
+  Next Obligation.
+    destruct x; intuition congruence.
+  Qed.
+
+  Program Definition aut: Syntax.t state header :=
+    {| t_states := states |}.
+  Solve Obligations with (destruct s; cbv; Lia.lia).
+End Plain.
+
+Module Optimized.
+Inductive state := | State_0_suff_1 | State_0_suff_3 | State_3 | State_0 | State_0_suff_2 | State_2 | State_3_suff_3 | State_3_suff_1 | State_1_suff_0 | State_3_suff_0 | State_1 | State_4 | State_3_suff_2 | State_2_suff_0.
 Scheme Equality for state.
 Global Instance state_eqdec: EquivDec.EqDec state eq := state_eq_dec.
 Global Program Instance state_finite: @Finite state _ state_eq_dec :=
-  {| enum := [ParseEth0; ParseEth1; ParseMPLS0; ParseMPLS1; ParseEoMPLS; ParseIPVer; ParseIPv4; ParseIPv6] |}.
+  {| enum := [State_0_suff_1; State_0_suff_3; State_3; State_0; State_0_suff_2; State_2; State_3_suff_3; State_3_suff_1; State_1_suff_0; State_3_suff_0; State_1; State_4; State_3_suff_2; State_2_suff_0] |}.
 Next Obligation.
 repeat constructor;
   repeat match goal with
@@ -216,7 +242,254 @@ Qed.
 Next Obligation.
   destruct x; intuition congruence.
 Qed.
+Inductive header : nat -> Type :=
+| buf_320: header 320
+| buf_128: header 128
+| buf_64: header 64
+| buf_112: header 112
+| buf_16: header 16
+| buf_304: header 304
+| buf_240: header 240
+| buf_144: header 144
+| buf_176: header 176
+| buf_208: header 208.
+Definition h320_eq_dec (x y: header 320) : {x = y} + {x <> y}.
+refine (
+  match x with
+  | buf_320 =>
+    match y with
+    | buf_320 => left eq_refl
+    end
+  end
+); unfold "<>"; intros H; inversion H.
+Defined.
+Definition h64_eq_dec (x y: header 64) : {x = y} + {x <> y}.
+refine (
+  match x with
+  | buf_64 =>
+    match y with
+    | buf_64 => left eq_refl
+    end
+  end
+); unfold "<>"; intros H; inversion H.
+Defined.
+Definition h128_eq_dec (x y: header 128) : {x = y} + {x <> y}.
+refine (
+  match x with
+  | buf_128 =>
+    match y with
+    | buf_128 => left eq_refl
+    end
+  end
+); unfold "<>"; intros H; inversion H.
+Defined.
+Definition h16_eq_dec (x y: header 16) : {x = y} + {x <> y}.
+refine (
+  match x with
+  | buf_16 =>
+    match y with
+    | buf_16 => left eq_refl
+    end
+  end
+); unfold "<>"; intros H; inversion H.
+Defined.
+Definition h112_eq_dec (x y: header 112) : {x = y} + {x <> y}.
+refine (
+  match x with
+  | buf_112 =>
+    match y with
+    | buf_112 => left eq_refl
+    end
+  end
+); unfold "<>"; intros H; inversion H.
+Defined.
+Definition h304_eq_dec (x y: header 304) : {x = y} + {x <> y}.
+refine (
+  match x with
+  | buf_304 =>
+    match y with
+    | buf_304 => left eq_refl
+    end
+  end
+); unfold "<>"; intros H; inversion H.
+Defined.
+Definition h240_eq_dec (x y: header 240) : {x = y} + {x <> y}.
+refine (
+  match x with
+  | buf_240 =>
+    match y with
+    | buf_240 => left eq_refl
+    end
+  end
+); unfold "<>"; intros H; inversion H.
+Defined.
+Definition h144_eq_dec (x y: header 144) : {x = y} + {x <> y}.
+refine (
+  match x with
+  | buf_144 =>
+    match y with
+    | buf_144 => left eq_refl
+    end
+  end
+); unfold "<>"; intros H; inversion H.
+Defined.
+Definition h176_eq_dec (x y: header 176) : {x = y} + {x <> y}.
+refine (
+  match x with
+  | buf_176 =>
+    match y with
+    | buf_176 => left eq_refl
+    end
+  end
+); unfold "<>"; intros H; inversion H.
+Defined.
+Definition h208_eq_dec (x y: header 208) : {x = y} + {x <> y}.
+refine (
+  match x with
+  | buf_208 =>
+    match y with
+    | buf_208 => left eq_refl
+    end
+  end
+); unfold "<>"; intros H; inversion H.
+Defined.
+Derive Signature for header.
+Definition header_eqdec_ (n: nat) (x: header n) (y: header n) : {x = y} + {x <> y}.
+  solve_header_eqdec_ n x y
+    ((existT (fun n => forall x y: header n, {x = y} + {x <> y}) _ h320_eq_dec) ::
+     (existT _ _ h64_eq_dec) ::
+     (existT _ _ h128_eq_dec) ::
+     (existT _ _ h16_eq_dec) ::
+     (existT _ _ h112_eq_dec) ::
+     (existT _ _ h304_eq_dec) ::
+     (existT _ _ h240_eq_dec) ::
+     (existT _ _ h144_eq_dec) ::
+     (existT _ _ h176_eq_dec) ::
+     (existT _ _ h208_eq_dec) ::
+      nil).
+Defined.
 
+Global Instance header_eqdec: forall n, EquivDec.EqDec (header n) eq := header_eqdec_.
+Global Instance header_eqdec': EquivDec.EqDec (Syntax.H' header) eq.
+  solve_eqdec'.
+Defined.
+Global Instance header_finite: forall n, @Finite (header n) _ _.
+  intros n; solve_indexed_finiteness n [320; 64 ; 128 ; 16 ; 112 ; 304 ; 240 ; 144 ; 176 ; 208 ].
+Qed.
+
+Global Program Instance header_finite': @Finite {n & header n} _ header_eqdec' :=
+  {| enum := [
+      existT _ _ buf_320
+    ; existT _ _ buf_128
+    ; existT _ _ buf_64
+    ; existT _ _ buf_112
+    ; existT _ _ buf_16
+    ; existT _ _ buf_304
+    ; existT _ _ buf_240
+    ; existT _ _ buf_144
+    ; existT _ _ buf_176
+    ; existT _ _ buf_208
+    ] |}.
+Next Obligation.
+  solve_header_finite.
+Qed.
+Next Obligation.
+dependent destruction X; subst;
+repeat (
+  match goal with
+  | |- ?L \/ ?R => (now left; trivial) || right
+  end
+).
+Qed.
+Definition states (s: state) :=
+  match s with
+  | State_0 => {|
+    st_op := extract(buf_112);
+    st_trans := transition select (| (EHdr buf_112)[15 -- 15], (EHdr buf_112)[14 -- 14], (EHdr buf_112)[13 -- 13], (EHdr buf_112)[12 -- 12], (EHdr buf_112)[11 -- 11], (EHdr buf_112)[10 -- 10], (EHdr buf_112)[9 -- 9], (EHdr buf_112)[8 -- 8], (EHdr buf_112)[7 -- 7], (EHdr buf_112)[6 -- 6], (EHdr buf_112)[5 -- 5], (EHdr buf_112)[4 -- 4], (EHdr buf_112)[3 -- 3], (EHdr buf_112)[2 -- 2], (EHdr buf_112)[1 -- 1], (EHdr buf_112)[0 -- 0], (EHdr buf_112)[111 -- 111], (EHdr buf_112)[110 -- 110], (EHdr buf_112)[109 -- 109], (EHdr buf_112)[108 -- 108], (EHdr buf_112)[107 -- 107], (EHdr buf_112)[106 -- 106], (EHdr buf_112)[105 -- 105], (EHdr buf_112)[104 -- 104], (EHdr buf_112)[103 -- 103], (EHdr buf_112)[102 -- 102], (EHdr buf_112)[101 -- 101], (EHdr buf_112)[100 -- 100], (EHdr buf_112)[99 -- 99], (EHdr buf_112)[98 -- 98], (EHdr buf_112)[97 -- 97], (EHdr buf_112)[96 -- 96], (EHdr buf_112)[15 -- 15], (EHdr buf_112)[14 -- 14], (EHdr buf_112)[13 -- 13], (EHdr buf_112)[12 -- 12], (EHdr buf_112)[11 -- 11], (EHdr buf_112)[10 -- 10], (EHdr buf_112)[9 -- 9], (EHdr buf_112)[8 -- 8], (EHdr buf_112)[7 -- 7], (EHdr buf_112)[6 -- 6], (EHdr buf_112)[5 -- 5], (EHdr buf_112)[4 -- 4], (EHdr buf_112)[3 -- 3], (EHdr buf_112)[2 -- 2], (EHdr buf_112)[1 -- 1], (EHdr buf_112)[0 -- 0], (EHdr buf_112)[15 -- 15], (EHdr buf_112)[14 -- 14], (EHdr buf_112)[13 -- 13], (EHdr buf_112)[12 -- 12], (EHdr buf_112)[11 -- 11], (EHdr buf_112)[10 -- 10], (EHdr buf_112)[9 -- 9], (EHdr buf_112)[8 -- 8], (EHdr buf_112)[7 -- 7], (EHdr buf_112)[6 -- 6], (EHdr buf_112)[5 -- 5], (EHdr buf_112)[4 -- 4], (EHdr buf_112)[3 -- 3], (EHdr buf_112)[2 -- 2], (EHdr buf_112)[1 -- 1], (EHdr buf_112)[0 -- 0]|) {{
+      (* [| *, *, *, *, *, *, *, *, *, *, *, *, *, *, *, *, exact #b|0, exact #b|0, exact #b|0, exact #b|0, exact #b|1, exact #b|0, exact #b|0, exact #b|0, exact #b|0, exact #b|0, exact #b|0, exact #b|0, exact #b|0, exact #b|0, exact #b|0, exact #b|0, *, *, *, *, *, *, *, *, *, *, *, *, *, *, *, *, *, *, *, *, *, *, *, *, *, *, *, *, *, *, *, * |] ==> accept ;;; *)
+      [| *, *, *, *, *, *, *, *, *, *, *, *, *, *, *, *, exact #b|1, exact #b|0, exact #b|0, exact #b|0, exact #b|0, exact #b|1, exact #b|1, exact #b|0, exact #b|1, exact #b|1, exact #b|0, exact #b|1, exact #b|1, exact #b|1, exact #b|0, exact #b|1, *, *, *, *, *, *, *, *, *, *, *, *, *, *, *, *, *, *, *, *, *, *, *, *, *, *, *, *, *, *, *, * |] ==> inl State_0_suff_1 ;;;
+      [| *, *, *, *, *, *, *, *, *, *, *, *, *, *, *, *, exact #b|1, exact #b|0, exact #b|0, exact #b|0, exact #b|1, exact #b|0, exact #b|0, exact #b|0, exact #b|0, exact #b|1, exact #b|0, exact #b|0, exact #b|0, exact #b|1, exact #b|1, exact #b|1, *, *, *, *, *, *, *, *, *, *, *, *, *, *, *, *, *, *, *, *, *, *, *, *, *, *, *, *, *, *, *, * |] ==> inl State_0_suff_2 ;;;
+      [| *, *, *, *, *, *, *, *, *, *, *, *, *, *, *, *, exact #b|1, exact #b|0, exact #b|0, exact #b|0, exact #b|1, exact #b|0, exact #b|0, exact #b|0, exact #b|0, exact #b|1, exact #b|0, exact #b|0, exact #b|1, exact #b|0, exact #b|0, exact #b|0, *, *, *, *, *, *, *, *, *, *, *, *, *, *, *, *, *, *, *, *, *, *, *, *, *, *, *, *, *, *, *, * |] ==> inl State_0_suff_3 ;;;
+      (* [| *, *, *, *, *, *, *, *, *, *, *, *, *, *, *, *, *, *, *, *, *, *, *, *, *, *, *, *, *, *, *, *, *, *, *, *, *, *, *, *, *, *, *, *, *, *, *, *, *, *, *, *, *, *, *, *, *, *, *, *, *, *, *, * |] ==> accept ;;; *)
+      reject
+    }}
+  |}
+  | State_0_suff_1 => {|
+    st_op := extract(buf_320);
+    st_trans := transition accept;
+  |}
+  | State_0_suff_2 => {|
+    st_op := extract(buf_16);
+    st_trans := transition inl State_2;
+  |}
+  | State_0_suff_3 => {|
+    st_op := extract(buf_16);
+    st_trans := transition inl State_3;
+  |}
+  | State_1 => {|
+    st_op := extract(buf_16);
+    st_trans := transition select (| (EHdr buf_16)[15 -- 15], (EHdr buf_16)[14 -- 14], (EHdr buf_16)[13 -- 13], (EHdr buf_16)[12 -- 12], (EHdr buf_16)[11 -- 11], (EHdr buf_16)[10 -- 10], (EHdr buf_16)[9 -- 9], (EHdr buf_16)[8 -- 8], (EHdr buf_16)[7 -- 7], (EHdr buf_16)[6 -- 6], (EHdr buf_16)[5 -- 5], (EHdr buf_16)[4 -- 4], (EHdr buf_16)[3 -- 3], (EHdr buf_16)[2 -- 2], (EHdr buf_16)[1 -- 1], (EHdr buf_16)[0 -- 0], (EHdr buf_16)[15 -- 15], (EHdr buf_16)[14 -- 14], (EHdr buf_16)[13 -- 13], (EHdr buf_16)[12 -- 12], (EHdr buf_16)[11 -- 11], (EHdr buf_16)[10 -- 10], (EHdr buf_16)[9 -- 9], (EHdr buf_16)[8 -- 8], (EHdr buf_16)[7 -- 7], (EHdr buf_16)[6 -- 6], (EHdr buf_16)[5 -- 5], (EHdr buf_16)[4 -- 4], (EHdr buf_16)[3 -- 3], (EHdr buf_16)[2 -- 2], (EHdr buf_16)[1 -- 1], (EHdr buf_16)[0 -- 0], (EHdr buf_16)[15 -- 15], (EHdr buf_16)[14 -- 14], (EHdr buf_16)[13 -- 13], (EHdr buf_16)[12 -- 12], (EHdr buf_16)[11 -- 11], (EHdr buf_16)[10 -- 10], (EHdr buf_16)[9 -- 9], (EHdr buf_16)[8 -- 8], (EHdr buf_16)[7 -- 7], (EHdr buf_16)[6 -- 6], (EHdr buf_16)[5 -- 5], (EHdr buf_16)[4 -- 4], (EHdr buf_16)[3 -- 3], (EHdr buf_16)[2 -- 2], (EHdr buf_16)[1 -- 1], (EHdr buf_16)[0 -- 0], (EHdr buf_16)[15 -- 15], (EHdr buf_16)[14 -- 14], (EHdr buf_16)[13 -- 13], (EHdr buf_16)[12 -- 12], (EHdr buf_16)[11 -- 11], (EHdr buf_16)[10 -- 10], (EHdr buf_16)[9 -- 9], (EHdr buf_16)[8 -- 8], (EHdr buf_16)[7 -- 7], (EHdr buf_16)[6 -- 6], (EHdr buf_16)[5 -- 5], (EHdr buf_16)[4 -- 4], (EHdr buf_16)[3 -- 3], (EHdr buf_16)[2 -- 2], (EHdr buf_16)[1 -- 1], (EHdr buf_16)[0 -- 0]|) {{
+      [| *, *, *, *, *, *, *, *, *, *, *, *, *, *, *, *, *, *, *, *, *, *, *, *, *, *, *, *, *, *, *, *, *, *, *, *, *, *, *, *, *, *, *, *, *, *, *, *, *, *, *, *, *, *, *, *, *, *, *, *, *, *, *, * |] ==> inl State_1_suff_0 ;;;
+      reject
+    }}
+  |}
+  | State_1_suff_0 => {|
+    st_op := extract(buf_128);
+    st_trans := transition accept;
+  |}
+  | State_2 => {|
+    st_op := extract(buf_16);
+    st_trans := transition select (| (EHdr buf_16)[15 -- 15], (EHdr buf_16)[14 -- 14], (EHdr buf_16)[13 -- 13], (EHdr buf_16)[12 -- 12], (EHdr buf_16)[11 -- 11], (EHdr buf_16)[10 -- 10], (EHdr buf_16)[9 -- 9], (EHdr buf_16)[8 -- 8], (EHdr buf_16)[7 -- 7], (EHdr buf_16)[6 -- 6], (EHdr buf_16)[5 -- 5], (EHdr buf_16)[4 -- 4], (EHdr buf_16)[3 -- 3], (EHdr buf_16)[2 -- 2], (EHdr buf_16)[1 -- 1], (EHdr buf_16)[0 -- 0], (EHdr buf_16)[15 -- 15], (EHdr buf_16)[14 -- 14], (EHdr buf_16)[13 -- 13], (EHdr buf_16)[12 -- 12], (EHdr buf_16)[11 -- 11], (EHdr buf_16)[10 -- 10], (EHdr buf_16)[9 -- 9], (EHdr buf_16)[8 -- 8], (EHdr buf_16)[7 -- 7], (EHdr buf_16)[6 -- 6], (EHdr buf_16)[5 -- 5], (EHdr buf_16)[4 -- 4], (EHdr buf_16)[3 -- 3], (EHdr buf_16)[2 -- 2], (EHdr buf_16)[1 -- 1], (EHdr buf_16)[0 -- 0], (EHdr buf_16)[15 -- 15], (EHdr buf_16)[14 -- 14], (EHdr buf_16)[13 -- 13], (EHdr buf_16)[12 -- 12], (EHdr buf_16)[11 -- 11], (EHdr buf_16)[10 -- 10], (EHdr buf_16)[9 -- 9], (EHdr buf_16)[8 -- 8], (EHdr buf_16)[7 -- 7], (EHdr buf_16)[6 -- 6], (EHdr buf_16)[5 -- 5], (EHdr buf_16)[4 -- 4], (EHdr buf_16)[3 -- 3], (EHdr buf_16)[2 -- 2], (EHdr buf_16)[1 -- 1], (EHdr buf_16)[0 -- 0], (EHdr buf_16)[15 -- 15], (EHdr buf_16)[14 -- 14], (EHdr buf_16)[13 -- 13], (EHdr buf_16)[12 -- 12], (EHdr buf_16)[11 -- 11], (EHdr buf_16)[10 -- 10], (EHdr buf_16)[9 -- 9], (EHdr buf_16)[8 -- 8], (EHdr buf_16)[7 -- 7], (EHdr buf_16)[6 -- 6], (EHdr buf_16)[5 -- 5], (EHdr buf_16)[4 -- 4], (EHdr buf_16)[3 -- 3], (EHdr buf_16)[2 -- 2], (EHdr buf_16)[1 -- 1], (EHdr buf_16)[0 -- 0]|) {{
+      [| *, *, *, *, *, *, *, *, *, *, *, *, *, *, *, *, *, *, *, *, *, *, *, *, *, *, *, *, *, *, *, *, *, *, *, *, *, *, *, *, *, *, *, *, *, *, *, *, *, *, *, *, *, *, *, *, *, *, *, *, *, *, *, * |] ==> inl State_2_suff_0 ;;;
+      reject
+    }}
+  |}
+  | State_2_suff_0 => {|
+    st_op := extract(buf_304);
+    st_trans := transition accept;
+  |}
+  | State_3 => {|
+    st_op := extract(buf_16);
+    st_trans := transition select (| (EHdr buf_16)[15 -- 15], (EHdr buf_16)[14 -- 14], (EHdr buf_16)[13 -- 13], (EHdr buf_16)[12 -- 12], (EHdr buf_16)[11 -- 11], (EHdr buf_16)[10 -- 10], (EHdr buf_16)[9 -- 9], (EHdr buf_16)[8 -- 8], (EHdr buf_16)[7 -- 7], (EHdr buf_16)[6 -- 6], (EHdr buf_16)[5 -- 5], (EHdr buf_16)[4 -- 4], (EHdr buf_16)[3 -- 3], (EHdr buf_16)[2 -- 2], (EHdr buf_16)[1 -- 1], (EHdr buf_16)[0 -- 0], (EHdr buf_16)[15 -- 15], (EHdr buf_16)[14 -- 14], (EHdr buf_16)[13 -- 13], (EHdr buf_16)[12 -- 12], (EHdr buf_16)[11 -- 11], (EHdr buf_16)[10 -- 10], (EHdr buf_16)[9 -- 9], (EHdr buf_16)[8 -- 8], (EHdr buf_16)[7 -- 7], (EHdr buf_16)[6 -- 6], (EHdr buf_16)[5 -- 5], (EHdr buf_16)[4 -- 4], (EHdr buf_16)[3 -- 3], (EHdr buf_16)[2 -- 2], (EHdr buf_16)[1 -- 1], (EHdr buf_16)[0 -- 0], (EHdr buf_16)[15 -- 15], (EHdr buf_16)[14 -- 14], (EHdr buf_16)[13 -- 13], (EHdr buf_16)[12 -- 12], (EHdr buf_16)[11 -- 11], (EHdr buf_16)[10 -- 10], (EHdr buf_16)[9 -- 9], (EHdr buf_16)[8 -- 8], (EHdr buf_16)[7 -- 7], (EHdr buf_16)[6 -- 6], (EHdr buf_16)[5 -- 5], (EHdr buf_16)[4 -- 4], (EHdr buf_16)[3 -- 3], (EHdr buf_16)[2 -- 2], (EHdr buf_16)[1 -- 1], (EHdr buf_16)[0 -- 0], (EHdr buf_16)[15 -- 15], (EHdr buf_16)[14 -- 14], (EHdr buf_16)[13 -- 13], (EHdr buf_16)[12 -- 12], (EHdr buf_16)[11 -- 11], (EHdr buf_16)[10 -- 10], (EHdr buf_16)[9 -- 9], (EHdr buf_16)[8 -- 8], (EHdr buf_16)[7 -- 7], (EHdr buf_16)[6 -- 6], (EHdr buf_16)[5 -- 5], (EHdr buf_16)[4 -- 4], (EHdr buf_16)[3 -- 3], (EHdr buf_16)[2 -- 2], (EHdr buf_16)[1 -- 1], (EHdr buf_16)[0 -- 0]|) {{
+      [| *, *, *, *, exact #b|0, exact #b|1, exact #b|0, exact #b|1, *, *, *, *, *, *, *, *, *, *, *, *, *, *, *, *, *, *, *, *, *, *, *, *, *, *, *, *, *, *, *, *, *, *, *, *, *, *, *, *, *, *, *, *, *, *, *, *, *, *, *, *, *, *, *, * |] ==> inl State_3_suff_0 ;;;
+      [| *, *, *, *, exact #b|0, exact #b|1, exact #b|1, exact #b|0, *, *, *, *, *, *, *, *, *, *, *, *, *, *, *, *, *, *, *, *, *, *, *, *, *, *, *, *, *, *, *, *, *, *, *, *, *, *, *, *, *, *, *, *, *, *, *, *, *, *, *, *, *, *, *, * |] ==> inl State_3_suff_1 ;;;
+      [| *, *, *, *, exact #b|0, exact #b|1, exact #b|1, exact #b|1, *, *, *, *, *, *, *, *, *, *, *, *, *, *, *, *, *, *, *, *, *, *, *, *, *, *, *, *, *, *, *, *, *, *, *, *, *, *, *, *, *, *, *, *, *, *, *, *, *, *, *, *, *, *, *, * |] ==> inl State_3_suff_2 ;;;
+      [| *, *, *, *, exact #b|1, exact #b|0, exact #b|0, exact #b|0, *, *, *, *, *, *, *, *, *, *, *, *, *, *, *, *, *, *, *, *, *, *, *, *, *, *, *, *, *, *, *, *, *, *, *, *, *, *, *, *, *, *, *, *, *, *, *, *, *, *, *, *, *, *, *, * |] ==> inl State_3_suff_3 ;;;
+      reject
+    }}
+  |}
+  | State_3_suff_0 => {|
+    st_op := extract(buf_144);
+    st_trans := transition accept;
+  |}
+  | State_3_suff_1 => {|
+    st_op := extract(buf_176);
+    st_trans := transition accept;
+  |}
+  | State_3_suff_2 => {|
+    st_op := extract(buf_208);
+    st_trans := transition accept;
+  |}
+  | State_3_suff_3 => {|
+    st_op := extract(buf_240);
+    st_trans := transition accept;
+  |}
+  | State_4 => {|
+    st_op := extract(buf_64);
+    st_trans := transition select (| (EHdr buf_64)[15 -- 15], (EHdr buf_64)[14 -- 14], (EHdr buf_64)[13 -- 13], (EHdr buf_64)[12 -- 12], (EHdr buf_64)[11 -- 11], (EHdr buf_64)[10 -- 10], (EHdr buf_64)[9 -- 9], (EHdr buf_64)[8 -- 8], (EHdr buf_64)[7 -- 7], (EHdr buf_64)[6 -- 6], (EHdr buf_64)[5 -- 5], (EHdr buf_64)[4 -- 4], (EHdr buf_64)[3 -- 3], (EHdr buf_64)[2 -- 2], (EHdr buf_64)[1 -- 1], (EHdr buf_64)[0 -- 0], (EHdr buf_64)[31 -- 31], (EHdr buf_64)[30 -- 30], (EHdr buf_64)[29 -- 29], (EHdr buf_64)[28 -- 28], (EHdr buf_64)[27 -- 27], (EHdr buf_64)[26 -- 26], (EHdr buf_64)[25 -- 25], (EHdr buf_64)[24 -- 24], (EHdr buf_64)[23 -- 23], (EHdr buf_64)[22 -- 22], (EHdr buf_64)[21 -- 21], (EHdr buf_64)[20 -- 20], (EHdr buf_64)[19 -- 19], (EHdr buf_64)[18 -- 18], (EHdr buf_64)[17 -- 17], (EHdr buf_64)[16 -- 16], (EHdr buf_64)[47 -- 47], (EHdr buf_64)[46 -- 46], (EHdr buf_64)[45 -- 45], (EHdr buf_64)[44 -- 44], (EHdr buf_64)[43 -- 43], (EHdr buf_64)[42 -- 42], (EHdr buf_64)[41 -- 41], (EHdr buf_64)[40 -- 40], (EHdr buf_64)[39 -- 39], (EHdr buf_64)[38 -- 38], (EHdr buf_64)[37 -- 37], (EHdr buf_64)[36 -- 36], (EHdr buf_64)[35 -- 35], (EHdr buf_64)[34 -- 34], (EHdr buf_64)[33 -- 33], (EHdr buf_64)[32 -- 32], (EHdr buf_64)[63 -- 63], (EHdr buf_64)[62 -- 62], (EHdr buf_64)[61 -- 61], (EHdr buf_64)[60 -- 60], (EHdr buf_64)[59 -- 59], (EHdr buf_64)[58 -- 58], (EHdr buf_64)[57 -- 57], (EHdr buf_64)[56 -- 56], (EHdr buf_64)[55 -- 55], (EHdr buf_64)[54 -- 54], (EHdr buf_64)[53 -- 53], (EHdr buf_64)[52 -- 52], (EHdr buf_64)[51 -- 51], (EHdr buf_64)[50 -- 50], (EHdr buf_64)[49 -- 49], (EHdr buf_64)[48 -- 48]|) {{
+      [| *, *, *, *, *, *, *, exact #b|0, *, *, *, *, *, *, *, *, *, *, *, *, *, *, *, *, *, *, *, *, *, *, *, *, *, *, *, *, *, *, *, exact #b|1, *, *, *, *, *, *, *, *, exact #b|0, exact #b|0, exact #b|0, exact #b|0, *, *, *, *, *, *, *, *, *, *, *, * |] ==> reject ;;;
+      [| *, *, *, *, *, *, *, exact #b|0, *, *, *, *, *, *, *, *, *, *, *, *, *, *, *, *, *, *, *, *, *, *, *, *, *, *, *, *, *, *, *, exact #b|1, *, *, *, *, *, *, *, *, exact #b|0, exact #b|1, exact #b|0, exact #b|0, *, *, *, *, *, *, *, *, *, *, *, * |] ==> reject ;;;
+      [| *, *, *, *, *, *, *, exact #b|0, *, *, *, *, *, *, *, *, *, *, *, *, *, *, *, *, *, *, *, *, *, *, *, *, *, *, *, *, *, *, *, exact #b|1, *, *, *, *, *, *, *, *, exact #b|0, exact #b|1, exact #b|1, exact #b|0, *, *, *, *, *, *, *, *, *, *, *, * |] ==> reject ;;;
+      [| *, *, *, *, *, *, *, exact #b|0, *, *, *, *, *, *, *, *, *, *, *, *, *, *, *, *, *, *, *, *, *, *, *, *, *, *, *, *, *, *, *, *, *, *, *, *, *, *, *, *, *, *, *, *, *, *, *, *, *, *, *, *, *, *, *, * |] ==> reject ;;;
+      [| *, *, *, *, *, *, *, exact #b|1, *, *, *, *, *, *, *, *, exact #b|0, exact #b|0, exact #b|0, exact #b|0, *, *, *, *, *, *, *, *, *, *, *, *, *, *, *, *, *, *, *, *, *, *, *, *, *, *, *, *, *, *, *, *, *, *, *, *, *, *, *, *, *, *, *, * |] ==> reject ;;;
+      [| *, *, *, *, *, *, *, exact #b|1, *, *, *, *, *, *, *, *, exact #b|0, exact #b|1, exact #b|0, exact #b|0, *, *, *, *, *, *, *, *, *, *, *, *, *, *, *, *, *, *, *, *, *, *, *, *, *, *, *, *, *, *, *, *, *, *, *, *, *, *, *, *, *, *, *, * |] ==> reject ;;;
+      [| *, *, *, *, *, *, *, exact #b|1, *, *, *, *, *, *, *, *, exact #b|0, exact #b|1, exact #b|1, exact #b|0, *, *, *, *, *, *, *, *, *, *, *, *, *, *, *, *, *, *, *, *, *, *, *, *, *, *, *, *, *, *, *, *, *, *, *, *, *, *, *, *, *, *, *, * |] ==> reject ;;;
+      [| *, *, *, *, *, *, *, *, *, *, *, *, *, *, *, *, *, *, *, *, *, *, *, *, *, *, *, *, *, *, *, *, *, *, *, *, *, *, *, *, *, *, *, *, *, *, *, *, *, *, *, *, *, *, *, *, *, *, *, *, *, *, *, * |] ==> reject ;;;
+      reject
+    }}
+  |}
+end.
 Program Definition aut: Syntax.t state header :=
   {| t_states := states |}.
 Solve Obligations with (destruct s; cbv; Lia.lia).
+End Optimized.
