deps/poulet4/lib/P4automata/Benchmarks/EdgeTransProof.v
@@ -1,0 +1,83 @@
+Require Import Poulet4.P4automata.Benchmarks.ProofHeader.
+Require Import Poulet4.P4automata.Benchmarks.Edge.
+
+Require Import Coq.Arith.PeanoNat.
+
+
+Declare ML Module "mirrorsolve".
+
+Notation H := (Plain.header + Optimized.header).
+Notation A := (Sum.sum Plain.aut Optimized.aut).
+Notation conf := (P4automaton.configuration (P4A.interp A)).
+Notation start_left := (Plain.ParseEth0).
+Notation start_right := (Optimized.State_0).
+
+Notation r_len := 7.
+(* Fixpoint reachable_states_len' (r: Reachability.state_pairs A) (acc: nat) (fuel: nat) :=
+  match fuel with
+  | 0 => None
+  | S x =>
+    let nxt := Reachability.reachable_step r in
+    let nxt_len := length nxt in
+    if Nat.eq_dec (length nxt) (length r) then Some acc
+    else
+      reachable_states_len' nxt (S acc) x
+  end.
+
+Definition reachable_states_len : nat.
+  refine (
+  let s := ({| st_state := inl (inl start_left); st_buf_len := 0 |},
+            {| st_state := inl (inr start_right); st_buf_len := 0 |}) in
+  let r := reachable_states_len' [s] 0 1000 in
+  _).
+  vm_compute in r.
+  match goal with
+  | _ := Some ?x |- _ => exact x
+  end.
+  Defined.
+Print reachable_states_len. *)
+
+Definition r_states : list (Reachability.state_pair A) :=
+  Eval vm_compute in (Reachability.reachable_states
+                        A
+                        r_len
+                        start_left
+                        start_right).
+
+Definition top : Relations.rel conf := fun _ _ => True.
+Definition top' : Relations.rel (state_template A) := fun _ _ => True.
+
+Lemma prebisim_babyip:
+  forall q1 q2,
+    interp_conf_rel' {| cr_st := {|
+                        cs_st1 := {|
+                          st_state := inl (inl start_left);
+                          st_buf_len := 0;
+                        |};
+                        cs_st2 := {|
+                          st_state := inl (inr start_right);
+                          st_buf_len := 0;
+                        |};
+                      |};
+                      cr_ctx := BCEmp;
+                      cr_rel := btrue;
+                  |} q1 q2 ->
+  pre_bisimulation A
+                  (wp r_states)
+                  top
+                  []
+                  (mk_init _ _ _ A r_len start_left start_right)
+                  q1 q2.
+Proof.
+  idtac "running edge translation validation".
+
+  intros.
+  set (rel0 := (mk_init _ _ _ _ _ _ _)).
+  vm_compute in rel0.
+  subst rel0.
+
+  time "build phase" repeat (time "single step" run_bisim top top' r_states).
+
+  (* run_bisim top top' r_states. *)
+  time "close phase" close_bisim top'.
+Time Admitted.
